theories/utp_csp.thy
@@ -2520,9 +2520,6 @@ qed
 lemma "\<lbrakk> \<And> a. P(a) is NCSP \<rbrakk> \<Longrightarrow> (\<box> x\<in>A \<^bold>\<rightarrow> P(x)) = (\<box> x\<in>A \<^bold>\<rightarrow> Skip) ;; (P x)\<lbrakk>x\<rightarrow>last\<^sub>u($tr)\<rbrakk>"
 *)
 
-lemma st_rel_RR: "[P]\<^sub>S is RR"
-  by (rel_auto)
-
 lemma RR_msubst_tt: "RR((P t)\<lbrakk>t\<rightarrow>&tt\<rbrakk>) = (RR (P t))\<lbrakk>t\<rightarrow>&tt\<rbrakk>"
   by (rel_auto)
 
@@ -2562,7 +2559,7 @@ lemma CRD_contract_refine:
   shows "[P\<^sub>1 \<turnstile> P\<^sub>2 trace refs | P\<^sub>3(trace)]\<^sub>C \<sqsubseteq> Q"
 proof -
   have "[P\<^sub>1 \<turnstile> P\<^sub>2 trace refs | P\<^sub>3(trace)]\<^sub>C \<sqsubseteq> \<^bold>R\<^sub>s(pre\<^sub>R(Q) \<turnstile> peri\<^sub>R(Q) \<diamondop> post\<^sub>R(Q))"
-    using assms by (simp add: mk_CRD_def, rule_tac srdes_tri_refine_intro, rel_auto+)
+    using assms by (simp add: mk_CRD_def, rule_tac srdes_tri_refine_intro, rel_auto+, blast)
   thus ?thesis
     by (simp add: SRD_reactive_tri_design assms(1))
 qed
@@ -3718,7 +3715,7 @@ qed
 lemma FinalMerge_csp_do [rpred]:
   assumes "vwb_lens ns1" "vwb_lens ns2" "ns1 \<bowtie> ns2"
   shows "\<Phi>(s\<^sub>1,\<sigma>\<^sub>1,t\<^sub>1) \<lbrakk>ns1|cs|ns2\<rbrakk>\<^sup>F \<Phi>(s\<^sub>2,\<sigma>\<^sub>2,t\<^sub>2) = 
-         ([s\<^sub>1 \<and> s\<^sub>2]\<^sub>S\<^sub>< \<and> [\<guillemotleft>trace\<guillemotright> \<in>\<^sub>u t\<^sub>1 \<star>\<^bsub>\<guillemotleft>cs\<guillemotright>\<^esub> t\<^sub>2 \<and> t\<^sub>1 \<restriction>\<^sub>u \<guillemotleft>cs\<guillemotright> =\<^sub>u t\<^sub>2 \<restriction>\<^sub>u \<guillemotleft>cs\<guillemotright>]\<^sub>t \<and> [\<langle>\<sigma>\<^sub>1 [&ns1|&ns2]\<^sub>s \<sigma>\<^sub>2\<rangle>\<^sub>a]\<^sub>S)" 
+         ([s\<^sub>1 \<and> s\<^sub>2]\<^sub>S\<^sub>< \<and> [\<guillemotleft>trace\<guillemotright> \<in>\<^sub>u t\<^sub>1 \<star>\<^bsub>\<guillemotleft>cs\<guillemotright>\<^esub> t\<^sub>2 \<and> t\<^sub>1 \<restriction>\<^sub>u \<guillemotleft>cs\<guillemotright> =\<^sub>u t\<^sub>2 \<restriction>\<^sub>u \<guillemotleft>cs\<guillemotright>]\<^sub>t \<and> [\<langle>\<sigma>\<^sub>1 [&ns1|&ns2]\<^sub>s \<sigma>\<^sub>2\<rangle>\<^sub>a]\<^sub>S')" 
   (is "?lhs = ?rhs")
 proof -
   have "?lhs = 
@@ -3729,7 +3726,7 @@ proof -
              $st\<acute> =\<^sub>u $st \<oplus> \<guillemotleft>st\<^sub>0\<guillemotright> on &ns1 \<oplus> \<guillemotleft>st\<^sub>1\<guillemotright> on &ns2)"
     by (simp add: CSPFinalMerge_form unrest closure assms)
   also have "... = 
-        ([s\<^sub>1 \<and> s\<^sub>2]\<^sub>S\<^sub>< \<and> [\<guillemotleft>trace\<guillemotright> \<in>\<^sub>u t\<^sub>1 \<star>\<^bsub>\<guillemotleft>cs\<guillemotright>\<^esub> t\<^sub>2 \<and> t\<^sub>1 \<restriction>\<^sub>u \<guillemotleft>cs\<guillemotright> =\<^sub>u t\<^sub>2 \<restriction>\<^sub>u \<guillemotleft>cs\<guillemotright>]\<^sub>t \<and> [\<langle>\<sigma>\<^sub>1 [&ns1|&ns2]\<^sub>s \<sigma>\<^sub>2\<rangle>\<^sub>a]\<^sub>S)"
+        ([s\<^sub>1 \<and> s\<^sub>2]\<^sub>S\<^sub>< \<and> [\<guillemotleft>trace\<guillemotright> \<in>\<^sub>u t\<^sub>1 \<star>\<^bsub>\<guillemotleft>cs\<guillemotright>\<^esub> t\<^sub>2 \<and> t\<^sub>1 \<restriction>\<^sub>u \<guillemotleft>cs\<guillemotright> =\<^sub>u t\<^sub>2 \<restriction>\<^sub>u \<guillemotleft>cs\<guillemotright>]\<^sub>t \<and> [\<langle>\<sigma>\<^sub>1 [&ns1|&ns2]\<^sub>s \<sigma>\<^sub>2\<rangle>\<^sub>a]\<^sub>S')"
     by (rel_auto)
   finally show ?thesis .
 qed
