utp/utp_lift.thy
@@ -32,12 +32,6 @@ where "\<lceil>P\<rceil>\<^sub>> \<equiv> P \<oplus>\<^sub>p snd\<^sub>L"
 abbreviation drop_post :: "('a, '\<alpha> \<times> '\<beta>) uexpr \<Rightarrow> ('a, '\<beta>) uexpr" ("\<lfloor>_\<rfloor>\<^sub>>")
 where "\<lfloor>P\<rfloor>\<^sub>> \<equiv> P \<restriction>\<^sub>e snd\<^sub>L"
   
-abbreviation lift_cond_pre ("\<lceil>_\<rceil>\<^sub>\<leftarrow>") where "\<lceil>P\<rceil>\<^sub>\<leftarrow> \<equiv> P \<oplus>\<^sub>p (1\<^sub>L \<times>\<^sub>L 0\<^sub>L)"
-abbreviation lift_cond_post ("\<lceil>_\<rceil>\<^sub>\<rightarrow>") where "\<lceil>P\<rceil>\<^sub>\<rightarrow> \<equiv> P \<oplus>\<^sub>p (0\<^sub>L \<times>\<^sub>L 1\<^sub>L)"
-
-abbreviation drop_cond_pre ("\<lfloor>_\<rfloor>\<^sub>\<leftarrow>") where "\<lfloor>P\<rfloor>\<^sub>\<leftarrow> \<equiv> P \<restriction>\<^sub>e (1\<^sub>L \<times>\<^sub>L 0\<^sub>L)"
-abbreviation drop_cond_post ("\<lfloor>_\<rfloor>\<^sub>\<rightarrow>") where "\<lfloor>P\<rfloor>\<^sub>\<rightarrow> \<equiv> P \<restriction>\<^sub>e (0\<^sub>L \<times>\<^sub>L 1\<^sub>L)"
-
 subsection {* Lifting Laws *}
 
 text {* With the help of our alphabet laws, we can prove some intuitive laws about alphabet
@@ -51,14 +45,6 @@ lemma lift_pre_var [simp]:
 lemma lift_post_var [simp]:
   "\<lceil>var x\<rceil>\<^sub>> = $x\<acute>"
   by (alpha_tac)
-
-lemma lift_cond_pre_var [simp]:
-  "\<lceil>$x\<rceil>\<^sub>\<leftarrow> = $x"
-  by (pred_auto)
-
-lemma lift_cond_post_var [simp]:
-  "\<lceil>$x\<acute>\<rceil>\<^sub>\<rightarrow> = $x\<acute>"
-  by (pred_auto)
 
 subsection {* Substitution Laws *}
     
@@ -77,8 +63,4 @@ lemma unrest_dash_var_pre [unrest]:
   shows "$x\<acute> \<sharp> \<lceil>p\<rceil>\<^sub><"
   by (pred_auto)
 
-lemma unrest_dash_var_cond_pre [unrest]:
-  fixes x :: "('a \<Longrightarrow> '\<alpha>)"
-  shows "$x\<acute> \<sharp> \<lceil>P\<rceil>\<^sub>\<leftarrow>"
-  by (pred_auto)
 end
